src/tls/Curve25519.fst
@@ -1,0 +1,46 @@
+(*--build-config
+options:--fstar_home ../../../FStar --max_fuel 4 --initial_fuel 0 --max_ifuel 2 --initial_ifuel 1 --z3rlimit 20 --__temp_no_proj Handshake --__temp_no_proj Connection --use_hints --include ../../../FStar/ucontrib/CoreCrypto/fst/ --include ../../../FStar/ucontrib/Platform/fst/ --include ../../../hacl-star/secure_api/LowCProvider/fst --include ../../../kremlin/kremlib --include ../../../hacl-star/specs --include ../../../hacl-star/code/lib/kremlin --include ../../../hacl-star/secure_api/test --include ../../../hacl-star/secure_api/utils --include ../../../hacl-star/secure_api/aead --include ../../libs/ffi --include ../../../FStar/ulib/hyperstack --include ../../src/tls/ideal-flags;
+--*)
+module Curve25519
+
+open FStar.Heap
+open FStar.HyperHeap
+open FStar.HyperStack
+open FStar.Seq
+
+open Platform.Bytes
+open Platform.Error
+
+module X = Spec.Curve25519
+module CC = CoreCrypto
+
+type scalar = lbytes 32
+type point = lbytes 32
+type keyshare = point * scalar
+
+let pubshare (k:keyshare) : Tot point = fst k
+
+// FIXME: Convert between Platform bytes (Seq.seq Char.char) and Hacl.Spec.Lib.bytes (Seq.seq UInt8.t)
+let bytes2hacl (b:bytes) : Tot (s:Seq.seq UInt8.t{Seq.length s = Seq.length b}) =
+  Seq.init (length b) (fun i ->
+    UInt8.uint_to_t (FStar.Char.int_of_char (Platform.Bytes.index b i)))
+
+let hacl2bytes (s:Seq.seq UInt8.t) : Tot (b:bytes{length b = Seq.length s}) =
+  Platform.Bytes.initBytes (Seq.length s) (fun i ->
+    FStar.Char.char_of_int (UInt8.v (Seq.index s i)))
+
+let point_of_scalar (s:scalar) : Tot point =
+  let base_point = Seq.upd (Seq.create 32 0uy) 0 9uy in
+  let p = X.scalarmult (bytes2hacl s) base_point in
+  hacl2bytes p
+
+let keygen () : ST keyshare
+  (requires (fun h0 -> True))
+  (ensures (fun h0 _ h1 -> modifies_none h0 h1))
+  =
+  let s : lbytes 32 = CC.random 32 in
+  (point_of_scalar s, s)
+
+let mul (k:scalar) (p:point) : Tot point =
+  let p = X.scalarmult (bytes2hacl k) (bytes2hacl p) in
+  hacl2bytes p
